riscv_model/code/ge_mod.dfy
@@ -1,6 +1,7 @@
 include "../spec/bv_ops.dfy"
 include "../spec/rsa_ops.dfy"
 include "../lib/powers.dfy"
+include "../../libraries/src/Collections/Sequences/LittleEndianNat.dfy"
 
 module ge_mod {
 
@@ -9,206 +10,210 @@ import opened bv_ops
 import opened rv_consts
 import opened rsa_ops
 
-// |A[..n]| == n, interp A[..n] as an int 
-function interp(A: seq<uint32>, n: nat) : nat
-    decreases n;
-    requires 0 <= n <= |A|;
-{
-    if n == 0 then 0
-    else word_interp(A, n - 1) + interp(A, n - 1)
-}
-
-lemma {:induction i} prefix_sum_lemma(S: seq<uint32>, S': seq<uint32>, i: nat)
-    requires 0 <= i <= |S| && 0 <= i <= |S'|;
-    requires S[..i] == S'[..i];
-    ensures interp(S, i) == interp(S', i);
-{
-    assert true;
-}
-        
-function word_interp(A: seq<uint32>, i: nat) : nat
-    requires i < |A|;
-{
-    A[i] as nat * postional_weight(i)
-}
-
-function postional_weight(i: nat) : nat
-{
-    power(BASE_32, i) as nat
-}
-
-lemma {:induction A} to_nat_upper_bound_lemma(A: seq<uint32>, n: nat)
-    requires |A| == n;
-    ensures to_nat(A) < pow_B32(|A|);
-{
-    if |A| == 0 {
-        reveal power();
-    } else {
-        ghost var A' := A[..(|A| - 1)];
-
-        calc ==> {
-            to_nat(A) == word_interp(A, |A| - 1) + interp(A, |A| - 1);
-            {
-                assert to_nat(A') == interp(A, |A| - 1) by {
-                    prefix_sum_lemma(A, A', |A| - 1);
-                }   
-            }
-            to_nat(A) == word_interp(A, |A| - 1) + to_nat(A');
-            {
-                assert to_nat(A') < power(BASE_32, |A'|) by {
-                    to_nat_upper_bound_lemma(A', |A'|);
-                }
-            }
-            to_nat(A) < word_interp(A, |A| - 1) + power(BASE_32, |A'|);
-            {
-                assert word_interp(A, |A| - 1) <= power(BASE_32, |A|) - power(BASE_32, |A| - 1) by {
-                    word_interp_upper_bound_lemma(A, |A| - 1);
-                }
-            }
-            to_nat(A) < power(BASE_32, |A|) - power(BASE_32, |A| - 1) + power(BASE_32, |A'|);
-            to_nat(A) < power(BASE_32, |A|);
-        }
-    }
-}
-
-lemma {:induction i} word_interp_upper_bound_lemma(A: seq<uint32>, i: nat)
-    requires i < |A|;
-    ensures word_interp(A, i) <= power(BASE_32, i + 1) - power(BASE_32, i);
-{
-    assert A[i] as int <= BASE_32;
-    calc ==> {
-        A[i] as int <= BASE_32;
-        A[i] as int * postional_weight(i) <= (BASE_32 - 1) * postional_weight(i);
-        {
-            assert word_interp(A, i) == A[i] as int * postional_weight(i);
-        }
-         word_interp(A, i) <= (BASE_32 - 1) * postional_weight(i);
-         word_interp(A, i) <= (BASE_32 - 1) * power(BASE_32, i);
-         word_interp(A, i) <= BASE_32 * power(BASE_32, i) - power(BASE_32, i);
-         {
-            power_add_one_lemma(BASE_32, i);
-         }
-         word_interp(A, i) <= power(BASE_32, i + 1) - power(BASE_32, i);
-    }
-}
-
-lemma cmp_msw_lemma(A: seq<uint32>, B: seq<uint32>)
-    requires |A| == |B| != 0;
-    ensures A[|A| - 1] > B[|B| - 1] ==> (to_nat(A) > to_nat(B));
-    ensures A[|A| - 1] < B[|B| - 1] ==> (to_nat(A) < to_nat(B));
-{
-    var n := |A|;
-    var A' := A[..n-1];
-    var B' := B[..n-1];
-    calc == {
-        to_nat(A) - to_nat(B);
-        {
-            prefix_sum_lemma(A, A', n - 1);
-            prefix_sum_lemma(B, B', n - 1);
-        }
-        interp(A', n - 1) +  word_interp(A, n - 1) - interp(B', n - 1) - word_interp(B, n - 1);
-        to_nat(A') - to_nat(B') + word_interp(A, n - 1) - word_interp(B, n - 1);
-        to_nat(A') - to_nat(B') + (A[n - 1] as int - B[n - 1] as int)  * postional_weight(n - 1);
-    }
-
-    if A[n - 1] > B[n - 1] {
-        calc >= {
-            to_nat(A') - to_nat(B') + (A[n - 1] as int - B[n - 1] as int)  * postional_weight(n - 1);
-            {
-                assert (A[n - 1] as int - B[n - 1] as int) >= 1;
-            }
-            to_nat(A') - to_nat(B') + postional_weight(n - 1);
-            {
-                assert to_nat(A') >= 0;
-            }
-            postional_weight(n - 1) - to_nat(B');
-            power(BASE_32, n - 1) - to_nat(B');
-        }
-
-        assert to_nat(B') < power(BASE_32, n - 1) by {
-            to_nat_upper_bound_lemma(B', n-1);
-        }
-
-        assert power(BASE_32, n - 1) - to_nat(B') > 0;
-        assert to_nat(A) > to_nat(B);
-    } else if A[n - 1] < B[n - 1] {
-        calc <= {
-            to_nat(A') - to_nat(B') + (A[n - 1] as int - B[n - 1] as int)  * postional_weight(n - 1);
-            {
-                assert (B[n - 1] as int - A[n - 1] as int) >= 1;
-            }
-            to_nat(A') - to_nat(B') - postional_weight(n - 1);
-            {
-                assert to_nat(B') >= 0;
-            }
-            to_nat(A') - postional_weight(n - 1);
-            to_nat(A') - power(BASE_32, n - 1);
-        }
-
-        assert to_nat(A') < power(BASE_32, n - 1) by {
-            to_nat_upper_bound_lemma(A', n-1);
-        }
-
-        assert to_nat(A') - power(BASE_32, n - 1) < 0;
-        assert to_nat(A) < to_nat(B);
-    }
-}
-
-lemma {:induction A, i} cmp_sufficient_lemma(A: seq<uint32>, B: seq<uint32>, i: nat)
-        requires 0 <= i < |A| == |B|;
-        requires forall j :: i < j < |A| ==> (A[j] == B[j]);
-        ensures A[i] > B[i] ==> (to_nat(A) > to_nat(B));
-        ensures A[i] < B[i] ==> (to_nat(A) < to_nat(B));
-    {
-        var n := |A|;
-        if n != 0 {
-            if i == n - 1 {
-                cmp_msw_lemma(A, B);
-            } else {
-                var n := |A|;
-                var A' := A[..n-1];
-                var B' := B[..n-1];
-
-                calc ==> {
-                    A[i] > B[i];
-                    {
-                        cmp_sufficient_lemma(A', B', i);
-                    }
-                    to_nat(A') > to_nat(B');
-                    {
-                        prefix_sum_lemma(A, A', n - 1);
-                        prefix_sum_lemma(B, B', n - 1);
-                    }
-                    interp(A, n - 1) > interp(B, n - 1);
-                    {
-                        assert word_interp(A, n - 1) == word_interp(B, n - 1);
-                    }
-                    interp(A, n - 1) +  word_interp(A, n - 1) > interp(B, n - 1) + word_interp(B, n - 1);
-                    to_nat(A) > to_nat(B);
-                }
-                assert A[i] > B[i] ==> (to_nat(A) > to_nat(B));
-
-                calc ==> {
-                    A[i] < B[i];
-                    {
-                        cmp_sufficient_lemma(A', B', i);
-                    }
-                    to_nat(A') < to_nat(B');
-                    {
-                        prefix_sum_lemma(A, A', n - 1);
-                        prefix_sum_lemma(B, B', n - 1);
-                    }
-                    interp(A, n - 1) < interp(B, n - 1);
-                    {
-                        assert word_interp(A, n - 1) == word_interp(B, n - 1);
-                    }
-                    interp(A, n - 1) +  word_interp(A, n - 1) < interp(B, n - 1) + word_interp(B, n - 1);
-                    to_nat(A) < to_nat(B);
-                }
-                assert A[i] < B[i] ==> (to_nat(A) < to_nat(B));
-            }
-        }
-    }
+import opened DivMod
+import opened Power
+import opened BoundedInts
+import opened BASE_32_Seq
+// 
+// function interp(A: seq<uint32>, n: nat) : nat
+//     decreases n;
+//     requires 0 <= n <= |A|;
+// {
+//     if n == 0 then 0
+//     else word_interp(A, n - 1) + interp(A, n - 1)
+// }
+// 
+// lemma {:induction i} prefix_sum_lemma(S: seq<uint32>, S': seq<uint32>, i: nat)
+//     requires 0 <= i <= |S| && 0 <= i <= |S'|;
+//     requires S[..i] == S'[..i];
+//     ensures interp(S, i) == interp(S', i);
+// {
+//     assert true;
+// }
+//         
+// function word_interp(A: seq<uint32>, i: nat) : nat
+//     requires i < |A|;
+// {
+//     A[i] as nat * postional_weight(i)
+// }
+// 
+// function postional_weight(i: nat) : nat
+// {
+//     power(BASE_32, i) as nat
+// }
+// 
+// lemma {:induction A} ToNatRight_upper_bound_lemma(A: seq<uint32>, n: nat)
+//     requires |A| == n;
+//     ensures ToNatRight(A) < pow_B32(|A|);
+// {
+//     if |A| == 0 {
+//         reveal power();
+//     } else {
+//         ghost var A' := A[..(|A| - 1)];
+// 
+//         calc ==> {
+//             ToNatRight(A) == word_interp(A, |A| - 1) + interp(A, |A| - 1);
+//             {
+//                 assert ToNatRight(A') == interp(A, |A| - 1) by {
+//                     prefix_sum_lemma(A, A', |A| - 1);
+//                 }   
+//             }
+//             ToNatRight(A) == word_interp(A, |A| - 1) + ToNatRight(A');
+//             {
+//                 assert ToNatRight(A') < power(BASE_32, |A'|) by {
+//                     ToNatRight_upper_bound_lemma(A', |A'|);
+//                 }
+//             }
+//             ToNatRight(A) < word_interp(A, |A| - 1) + power(BASE_32, |A'|);
+//             {
+//                 assert word_interp(A, |A| - 1) <= power(BASE_32, |A|) - power(BASE_32, |A| - 1) by {
+//                     word_interp_upper_bound_lemma(A, |A| - 1);
+//                 }
+//             }
+//             ToNatRight(A) < power(BASE_32, |A|) - power(BASE_32, |A| - 1) + power(BASE_32, |A'|);
+//             ToNatRight(A) < power(BASE_32, |A|);
+//         }
+//     }
+// }
+// 
+// lemma {:induction i} word_interp_upper_bound_lemma(A: seq<uint32>, i: nat)
+//     requires i < |A|;
+//     ensures word_interp(A, i) <= power(BASE_32, i + 1) - power(BASE_32, i);
+// {
+//     assert A[i] as int <= BASE_32;
+//     calc ==> {
+//         A[i] as int <= BASE_32;
+//         A[i] as int * postional_weight(i) <= (BASE_32 - 1) * postional_weight(i);
+//         {
+//             assert word_interp(A, i) == A[i] as int * postional_weight(i);
+//         }
+//          word_interp(A, i) <= (BASE_32 - 1) * postional_weight(i);
+//          word_interp(A, i) <= (BASE_32 - 1) * power(BASE_32, i);
+//          word_interp(A, i) <= BASE_32 * power(BASE_32, i) - power(BASE_32, i);
+//          {
+//             power_add_one_lemma(BASE_32, i);
+//          }
+//          word_interp(A, i) <= power(BASE_32, i + 1) - power(BASE_32, i);
+//     }
+// }
+// 
+// lemma cmp_msw_lemma(A: seq<uint32>, B: seq<uint32>)
+//     requires |A| == |B| != 0;
+//     ensures A[|A| - 1] > B[|B| - 1] ==> (ToNatRight(A) > ToNatRight(B));
+//     ensures A[|A| - 1] < B[|B| - 1] ==> (ToNatRight(A) < ToNatRight(B));
+// {
+//     var n := |A|;
+//     var A' := A[..n-1];
+//     var B' := B[..n-1];
+//     calc == {
+//         ToNatRight(A) - ToNatRight(B);
+//         {
+//             prefix_sum_lemma(A, A', n - 1);
+//             prefix_sum_lemma(B, B', n - 1);
+//         }
+//         interp(A', n - 1) +  word_interp(A, n - 1) - interp(B', n - 1) - word_interp(B, n - 1);
+//         ToNatRight(A') - ToNatRight(B') + word_interp(A, n - 1) - word_interp(B, n - 1);
+//         ToNatRight(A') - ToNatRight(B') + (A[n - 1] as int - B[n - 1] as int)  * postional_weight(n - 1);
+//     }
+// 
+//     if A[n - 1] > B[n - 1] {
+//         calc >= {
+//             ToNatRight(A') - ToNatRight(B') + (A[n - 1] as int - B[n - 1] as int)  * postional_weight(n - 1);
+//             {
+//                 assert (A[n - 1] as int - B[n - 1] as int) >= 1;
+//             }
+//             ToNatRight(A') - ToNatRight(B') + postional_weight(n - 1);
+//             {
+//                 assert ToNatRight(A') >= 0;
+//             }
+//             postional_weight(n - 1) - ToNatRight(B');
+//             power(BASE_32, n - 1) - ToNatRight(B');
+//         }
+// 
+//         assert ToNatRight(B') < power(BASE_32, n - 1) by {
+//             ToNatRight_upper_bound_lemma(B', n-1);
+//         }
+// 
+//         assert power(BASE_32, n - 1) - ToNatRight(B') > 0;
+//         assert ToNatRight(A) > ToNatRight(B);
+//     } else if A[n - 1] < B[n - 1] {
+//         calc <= {
+//             ToNatRight(A') - ToNatRight(B') + (A[n - 1] as int - B[n - 1] as int)  * postional_weight(n - 1);
+//             {
+//                 assert (B[n - 1] as int - A[n - 1] as int) >= 1;
+//             }
+//             ToNatRight(A') - ToNatRight(B') - postional_weight(n - 1);
+//             {
+//                 assert ToNatRight(B') >= 0;
+//             }
+//             ToNatRight(A') - postional_weight(n - 1);
+//             ToNatRight(A') - power(BASE_32, n - 1);
+//         }
+// 
+//         assert ToNatRight(A') < power(BASE_32, n - 1) by {
+//             ToNatRight_upper_bound_lemma(A', n-1);
+//         }
+// 
+//         assert ToNatRight(A') - power(BASE_32, n - 1) < 0;
+//         assert ToNatRight(A) < ToNatRight(B);
+//     }
+// }
+// 
+// lemma {:induction A, i} cmp_sufficient_lemma(A: seq<uint32>, B: seq<uint32>, i: nat)
+//         requires 0 <= i < |A| == |B|;
+//         requires forall j :: i < j < |A| ==> (A[j] == B[j]);
+//         ensures A[i] > B[i] ==> (ToNatRight(A) > ToNatRight(B));
+//         ensures A[i] < B[i] ==> (ToNatRight(A) < ToNatRight(B));
+//     {
+//         var n := |A|;
+//         if n != 0 {
+//             if i == n - 1 {
+//                 cmp_msw_lemma(A, B);
+//             } else {
+//                 var n := |A|;
+//                 var A' := A[..n-1];
+//                 var B' := B[..n-1];
+// 
+//                 calc ==> {
+//                     A[i] > B[i];
+//                     {
+//                         cmp_sufficient_lemma(A', B', i);
+//                     }
+//                     ToNatRight(A') > ToNatRight(B');
+//                     {
+//                         prefix_sum_lemma(A, A', n - 1);
+//                         prefix_sum_lemma(B, B', n - 1);
+//                     }
+//                     interp(A, n - 1) > interp(B, n - 1);
+//                     {
+//                         assert word_interp(A, n - 1) == word_interp(B, n - 1);
+//                     }
+//                     interp(A, n - 1) +  word_interp(A, n - 1) > interp(B, n - 1) + word_interp(B, n - 1);
+//                     ToNatRight(A) > ToNatRight(B);
+//                 }
+//                 assert A[i] > B[i] ==> (ToNatRight(A) > ToNatRight(B));
+// 
+//                 calc ==> {
+//                     A[i] < B[i];
+//                     {
+//                         cmp_sufficient_lemma(A', B', i);
+//                     }
+//                     ToNatRight(A') < ToNatRight(B');
+//                     {
+//                         prefix_sum_lemma(A, A', n - 1);
+//                         prefix_sum_lemma(B, B', n - 1);
+//                     }
+//                     interp(A, n - 1) < interp(B, n - 1);
+//                     {
+//                         assert word_interp(A, n - 1) == word_interp(B, n - 1);
+//                     }
+//                     interp(A, n - 1) +  word_interp(A, n - 1) < interp(B, n - 1) + word_interp(B, n - 1);
+//                     ToNatRight(A) < ToNatRight(B);
+//                 }
+//                 assert A[i] < B[i] ==> (ToNatRight(A) < ToNatRight(B));
+//             }
+//         }
+//     }
 
         
 lemma ge_to_nat(a: seq<uint32>, n: seq<uint32>, i: nat)
@@ -216,21 +221,22 @@ lemma ge_to_nat(a: seq<uint32>, n: seq<uint32>, i: nat)
   requires i < |a|
   requires a[i] < n[i]
   requires forall j :: i < j < |a| ==> a[j] == n[j]
-  ensures to_nat(a) < to_nat(n)
+  ensures ToNatRight(a) < ToNatRight(n)
 {
-  cmp_sufficient_lemma(a, n, i);
+  // cmp_sufficient_lemma(a, n, i);
+  LemmaSeqMswInequality(a, n);
   calc {
-    to_nat(a[..i] + [a[i]] + a[i+1..]) < to_nat(n[..i] + [n[i]] + n[i+1..]);
+    ToNatRight(a[..i] + [a[i]] + a[i+1..]) < ToNatRight(n[..i] + [n[i]] + n[i+1..]);
     { assert a[..i] + [a[i]] + a[i+1..] == a;
       assert n[..i] + [n[i]] + n[i+1..] == n;
     }
-    to_nat(a) < to_nat(n);
+    ToNatRight(a) < ToNatRight(n);
   }
 }
 
   method ge_mod(a: seq<uint32>, n: seq<uint32>) returns (b:bool)
     requires |a| == |n| == 384
-    ensures (to_nat(a) >= to_nat(n)) == b
+    ensures (ToNatRight(a) >= ToNatRight(n)) == b
   {
     var i := |a| - 1;
 
@@ -243,7 +249,7 @@ lemma ge_to_nat(a: seq<uint32>, n: seq<uint32>, i: nat)
       invariant cond == 1 ==> a[i+1..] == n[i+1..]
       invariant !b ==> cond == 0;
       invariant cond == 0 ==> (b ==> a[i+1] > n[i+1]) || (a == n)
-      invariant cond == 0 ==> (to_nat(a) >= to_nat(n)) == b
+      invariant cond == 0 ==> (ToNatRight(a) >= ToNatRight(n)) == b
       decreases i
     {
 
